

Solve the system of equations.

$$\begin{cases} 3x + 6y = -9 \\ -x - 2y = 3 \\ -\frac{1}{2}x - y = \frac{3}{2} \end{cases}$$

☐ $[x = -3, y = 0]$

☐ $[x = -2a + 3, y = a, a \text{ is any real number}]$

☐ *no solution*

☐ $[x = -2a - 3, y = a, a \text{ is any real number}]$

☐ $\left[x = 0, y = -\frac{3}{2} \right]$

Give the solution set to the system of equations

$$\begin{cases} x - 4y + 2z = -1 \\ -4x + 2y - 2z = 2 \\ -2x + y - z = 2 \end{cases}$$

☐ $\left[x = \frac{3}{2} - \frac{11}{2}s, y = \frac{3}{2} - \frac{7}{2}s, z = -\frac{9}{2} - \frac{1}{2}s \right]$

☐ $\left[x = -\frac{1}{2} - \frac{13}{2}s, y = -\frac{1}{2} - \frac{1}{2}s, z = -\frac{7}{2} - \frac{11}{2}s \right]$

☐ $\left[x = -\frac{7}{2} - \frac{1}{2}s, y = \frac{5}{2} + \frac{3}{2}s, z = -\frac{7}{2} - \frac{1}{2}s \right]$

☐ *The system does not have a solution.*

☐ $\left[x = \frac{1}{2} - \frac{13}{2}s, y = -\frac{1}{2} - \frac{7}{2}s, z = -\frac{7}{2} - \frac{1}{2}s \right]$

Which of the following gives the correct matrix for this system of equations in reduced row echelon form?

$$\begin{cases} 3x_1 - 4x_2 + x_3 + 2x_4 = -3 \\ -2x_1 + 2x_2 - 3x_3 = -4 \\ 3x_1 - 2x_2 + 4x_3 + 2x_4 = -2 \end{cases}$$

☐ $\begin{bmatrix} 1 & 0 & 0 & \frac{17}{27} & \frac{50}{27} \\ 0 & 1 & 0 & \frac{47}{54} & \frac{4}{27} \\ 0 & 0 & 1 & \frac{11}{27} & \frac{53}{27} \end{bmatrix}$

☐ $\begin{bmatrix} 1 & 0 & 0 & 3 & \frac{38}{5} \\ 0 & 1 & 0 & \frac{3}{2} & \frac{28}{5} \\ 0 & 0 & 1 & -1 & -\frac{17}{5} \end{bmatrix}$

☐ $\begin{bmatrix} -3 & -4 & -1 & 2 & -3 \\ 0 & \frac{14}{3} & \frac{2}{3} & -\frac{13}{3} & -2 \\ 0 & 0 & \frac{27}{7} & -\frac{11}{7} & -\frac{53}{7} \end{bmatrix}$

☐ $\begin{bmatrix} 3 & -4 & 1 & 2 & -3 \\ 0 & -\frac{2}{3} & \frac{2}{3} & -\frac{5}{3} & -6 \\ 0 & 0 & 5 & -5 & -17 \end{bmatrix}$

☐ $\begin{bmatrix} 1 & 0 & 0 & \frac{1}{3} & \frac{10}{21} \\ 0 & 1 & 0 & -\frac{5}{6} & -\frac{22}{21} \\ 0 & 0 & 1 & \frac{1}{6} & -\frac{29}{21} \end{bmatrix}$

For what values of a does the system below have nontrivial solutions?

$$\begin{cases} 3x + 3y - 2z = 0 \\ -6x + ay + 4z = 0 \\ 2x + 4y + 4z = 0 \end{cases}$$

☐ -2

☐ 6

☐ 2

☐ -6

☐ 3

Given:

$$A = \begin{bmatrix} -3 & 3 \\ 3 & 5 \\ 5 & 3 \end{bmatrix} \quad B = \begin{bmatrix} -2 & 3 \\ -4 & -1 \\ -1 & 2 \end{bmatrix} \quad C = \begin{bmatrix} -3 & -2 \\ -3 & 1 \end{bmatrix} \quad D = \begin{bmatrix} 5 & 1 \\ 5 & 6 \end{bmatrix}$$

Compute $3CD - 2D$.

☐ *Not possible.*

☐ $\begin{bmatrix} -75 & -45 \\ -30 & 9 \end{bmatrix}$

☐ $\begin{bmatrix} -85 & -48 \\ -41 & -3 \end{bmatrix}$

☐ $\begin{bmatrix} -85 & -47 \\ -40 & -3 \end{bmatrix}$

☐ $\begin{bmatrix} -19 & -9 \\ -20 & -9 \end{bmatrix}$

The matrices A and B are given by

$$A = \begin{bmatrix} 1 & -2 & 3 \\ 0 & 2 & -1 \\ 1 & -3 & 0 \end{bmatrix} \quad B = \begin{bmatrix} 1 & -3 & -1 \\ -2 & 2 & 1 \\ 2 & -2 & 1 \end{bmatrix}$$

and $D = AB$. Give the value of $d_{2,1}$.

☐ -4

☐ -3

☐ -6

☐ -1

☐ -8

The matrices A, B and C are given by

$$A = \begin{bmatrix} -2 & 3 \\ -2 & 2 \\ -1 & -2 \end{bmatrix} \quad B = \begin{bmatrix} 2 & 3 & 0 \\ -2 & -3 & 2 \end{bmatrix} \quad C = \begin{bmatrix} 3 & -3 & 1 \\ -2 & -3 & 2 \\ 0 & -2 & -3 \end{bmatrix}$$

and $D = AB - 3C$. Give the value of $d_{2,3}$.

- ☐ 1
- ☐ -2
- ☐ 10
- ☐ 9
- ☐ -4

Let

$$A = \begin{bmatrix} -2 & -3 & 1 \\ 0 & -1 & 2 \\ 3 & 3 & 1 \end{bmatrix}$$

Find A^{-1} , if it exists.

☐ $\begin{bmatrix} 9 & -8 & 7 \\ -7 & 7 & -3 \\ -3 & 5 & -1 \end{bmatrix}$

☐ $\begin{bmatrix} 6 & -7 & 4 \\ -4 & 5 & -5 \\ -2 & 3 & -3 \end{bmatrix}$

☐ *A does not have an inverse.*

☐ $\begin{bmatrix} 7 & -6 & 5 \\ -6 & 5 & -4 \\ -3 & 3 & -2 \end{bmatrix}$

☐ $\begin{bmatrix} 6 & -4 & 7 \\ -5 & 5 & -3 \\ -2 & 5 & -2 \end{bmatrix}$

Use Cramer's rule to give the value of y for the solution set to the system of equations

$$\begin{cases} 4x - 5y - 2z = 1 \\ -x + 3y + 2z = -1 \\ -x + 2y + z = -2 \end{cases}$$

☐ $y = -12$

☐ $y = -9$

☐ $y = -8$

☐ $y = -11$

☐ *The system does not have a solution.*

Determine the values of λ for which the system below has nontrivial solutions.

$$\begin{cases} (4 - \lambda)x + 5y = 0 \\ 6x + (5 - \lambda)y = 0 \end{cases}$$

☐ $\lambda = \{0, 11\}$

☐ $\lambda = \{-1, 10\}$

☐ $\lambda = \{-2, 8\}$

☐ $\lambda = \{4, 5\}$

☐ $\lambda = \{-11, -1\}$

Find the eigenvalues and number of independent eigenvectors. (Hint: 4 is an eigenvalue.)

$$\begin{bmatrix} 10 & -6 & 0 \\ 12 & -8 & 0 \\ 12 & -5 & -3 \end{bmatrix}$$

- ☐ Eigenvalues: 4, 2, -3; Number of independent eigenvectors: 3
- ☐ Eigenvalues: 4, 4, -3; Number of independent eigenvectors: 2
- ☐ Eigenvalues: 4, -2, -2; Number of independent eigenvectors: 2
- ☐ Eigenvalues: 4, -2, 3; Number of independent eigenvectors: 3
- ☐ Eigenvalues: 4, -2, -3; Number of independent eigenvectors: 3

Find the eigenvalues and number of independent eigenvectors. (Hint: 3 is an eigenvalue.)

$$\begin{bmatrix} 1 & 0 & 1 \\ -2 & 2 & 2 \\ -2 & -1 & 5 \end{bmatrix}$$

- ☐ Eigenvalues: 3, 3, 2; Number of independent eigenvectors: 2
- ☐ Eigenvalues: -3, -3, 2; Number of independent eigenvectors: 2
- ☐ Eigenvalues: 3, -3, 2; Number of independent eigenvectors: 3
- ☐ Eigenvalues: 3, 2, -2; Number of independent eigenvectors: 3
- ☐ Eigenvalues: 3, 2, 2; Number of independent eigenvectors: 3

Question number 13. (5.00 points)

Given the linear differential system $\mathbf{x}' = A \mathbf{x}$ with

$$A = \begin{bmatrix} -2 & -3 \\ -8 & 0 \end{bmatrix}$$

Determine if \mathbf{u}, \mathbf{v} form a fundamental solution set. If so, give the general solution to the system.

$$\mathbf{u} = \begin{bmatrix} -2e^{4t} \\ 4e^{4t} \end{bmatrix}, \quad \mathbf{v} = \begin{bmatrix} 4e^{4t} \\ -8e^{4t} \end{bmatrix}$$

☐ $\begin{bmatrix} x_1 \\ x_2 \end{bmatrix} = C_1 \begin{bmatrix} -2e^{4t} \\ 4e^{4t} \end{bmatrix} + C_2 \begin{bmatrix} 4e^{4t} \\ -8e^{4t} \end{bmatrix}$

☐ $\begin{bmatrix} x_1 \\ x_2 \end{bmatrix} = C \begin{bmatrix} e^t \\ e^t \end{bmatrix} + C \begin{bmatrix} e^{\frac{13}{8}t} \\ -e^{\frac{13}{8}t} \end{bmatrix}$

☐ $\begin{bmatrix} x_1 \\ x_2 \end{bmatrix} = C_1 \begin{bmatrix} e^{4t} \\ -2e^{4t} \end{bmatrix} + C_2 \begin{bmatrix} -2e^{4t} \\ 4e^{4t} \end{bmatrix}$

☐ Not a fundamental solution set.

☐ $\begin{bmatrix} x_1 \\ x_2 \end{bmatrix} = \begin{bmatrix} -2e^{4t} \\ 4e^{4t} \end{bmatrix} + \begin{bmatrix} 4e^{4t} \\ -8e^{4t} \end{bmatrix}$

Find the general solution to the system $\mathbf{x}' = A \mathbf{x}$ where A is the given matrix.

$$A = \begin{bmatrix} 2 & 2 \\ 2 & 5 \end{bmatrix}$$

☐ $\mathbf{x}(t) = C_1 e^{6t} \begin{bmatrix} -2 \\ 1 \end{bmatrix} + C_2 e^t \begin{bmatrix} 1 \\ 2 \end{bmatrix}$

☐ $\mathbf{x}(t) = C_1 e^{6t} \begin{bmatrix} -2 \\ 1 \end{bmatrix} + C_2 e^{-t} \begin{bmatrix} 2 \\ -2 \end{bmatrix}$

☐ $\mathbf{x}(t) = C_1 e^{6t} \begin{bmatrix} 1 \\ 2 \end{bmatrix} + C_2 e^t \begin{bmatrix} -2 \\ 1 \end{bmatrix}$

☐ $\mathbf{x}(t) = C_1 e^{-6t} \begin{bmatrix} 2 \\ -2 \end{bmatrix} + C_2 e^{-t} \begin{bmatrix} -2 \\ 1 \end{bmatrix}$

☐ $\mathbf{x}(t) = C_1 e^{-6t} \begin{bmatrix} 2 \\ -2 \end{bmatrix} + C_2 e^t \begin{bmatrix} 2 \\ 5 \end{bmatrix}$

Question number 15. (5.00 points)

Give the value(s) of a for which the columns in the matrix

$$A = \begin{bmatrix} 10 & -6 & -9+a \\ -6 & 18 & 9 \\ -9+a & 9 & 9 \end{bmatrix}$$

are linearly dependent.

☐ {2, 15}

☐ {-1, 13}

☐ {3, 14}

☐ {2, 11}

☐ {0, 12}

☐ None of the above.

Question number 16. (5.00 points)

Find a fundamental set of solution vectors of the system $\mathbf{x}' = A \mathbf{x}$ where A is the given matrix:

$$A = \begin{bmatrix} 2 & -3 & 4 \\ -2 & 5 & -4 \\ 0 & 3 & -2 \end{bmatrix}$$

and find the solution that satisfies the initial condition:

$$\mathbf{x}(0) = \begin{bmatrix} -2 \\ 1 \\ 0 \end{bmatrix}$$

Hint: -1 is an eigenvalue.

☐ $\mathbf{x}(t) = \frac{9}{5} e^{-2t} \begin{bmatrix} 4 \\ 3 \\ -2 \end{bmatrix} + \frac{9}{5} e^{4t} \begin{bmatrix} 2 \\ -2 \\ 0 \end{bmatrix} + \frac{1}{15} e^{-t} \begin{bmatrix} 2 \\ -4 \\ -3 \end{bmatrix}$

☐ $\mathbf{x}(t) = -\frac{4}{3} e^{2t} \begin{bmatrix} -1 \\ 2 \\ 1 \end{bmatrix} + \frac{18}{5} e^{5t} \begin{bmatrix} 0 \\ 4 \\ 3 \end{bmatrix} + \frac{1}{15} e^{-t} \begin{bmatrix} -3 \\ 1 \\ 3 \end{bmatrix}$

☐ $\mathbf{x}(t) = \frac{2}{3} e^{2t} \begin{bmatrix} -1 \\ 2 \\ 1 \end{bmatrix} + \frac{9}{5} e^{-5t} \begin{bmatrix} 2 \\ -4 \\ -3 \end{bmatrix} - \frac{2}{3} e^{-t} \begin{bmatrix} 2 \\ -4 \\ -3 \end{bmatrix}$

☐ $\mathbf{x}(t) = -\frac{4}{3} e^{-2t} \begin{bmatrix} 2 \\ 3 \\ 4 \end{bmatrix} - \frac{4}{3} e^{-4t} \begin{bmatrix} -1 \\ 2 \\ 1 \end{bmatrix} + \frac{1}{15} e^{-t} \begin{bmatrix} 1 \\ 1 \\ 1 \end{bmatrix}$

☐ $\mathbf{x}(t) = -\frac{2}{3} e^{2t} \begin{bmatrix} 0 \\ 4 \\ 3 \end{bmatrix} + \frac{9}{5} e^{4t} \begin{bmatrix} -1 \\ 2 \\ 1 \end{bmatrix} + \frac{1}{15} e^{-t} \begin{bmatrix} -3 \\ 1 \\ 3 \end{bmatrix}$

☐ None of the above

Find the general solution to the system $\mathbf{x}' = A \mathbf{x}$ where A is the given matrix.

$$A = \begin{bmatrix} 4 & 3 \\ -3 & -2 \end{bmatrix}$$

☐ $\mathbf{x}(t) = C_1 e^{-t} \begin{bmatrix} -1 \\ 0 \end{bmatrix} + C_2 \left(e^{-t} \begin{bmatrix} -1 \\ 0 \end{bmatrix} + t e^{-t} \begin{bmatrix} -1 \\ 1 \end{bmatrix} \right)$

☐ $\mathbf{x}(t) = C_1 e^t \begin{bmatrix} -1 \\ 1 \end{bmatrix} + C_2 \left(e^t \begin{bmatrix} -1 \\ 0 \end{bmatrix} + t e^t \begin{bmatrix} -1 \\ 1 \end{bmatrix} \right)$

☐ $\mathbf{x}(t) = C_1 e^t \begin{bmatrix} -1 \\ 1 \end{bmatrix} + C_2 \left(e^t \begin{bmatrix} -1 \\ 1 \end{bmatrix} + t e^t \begin{bmatrix} -1 \\ 0 \end{bmatrix} \right)$

☐ $\mathbf{x}(t) = C_1 e^{-t} \begin{bmatrix} 1 \\ 1 \end{bmatrix} + C_2 t e^t \begin{bmatrix} -1 \\ 0 \end{bmatrix}$

☐ $\mathbf{x}(t) = C_1 e^t \begin{bmatrix} 1 \\ 1 \end{bmatrix} + C_2 t e^t \begin{bmatrix} -1 \\ 0 \end{bmatrix}$

Find the general solution to the system $\mathbf{x}' = A \mathbf{x}$ where A is the given matrix.

$$A = \begin{bmatrix} 3 & 3 \\ -3 & 3 \end{bmatrix}$$

☐ $\mathbf{x}(t) = C_1 e^{3t} \begin{pmatrix} \cos(3t) \begin{bmatrix} 1 \\ 0 \end{bmatrix} - \sin(3t) \begin{bmatrix} -1 \\ 0 \end{bmatrix} \end{pmatrix} + C_2 e^{-3t} \begin{pmatrix} \cos(3t) \begin{bmatrix} -1 \\ 0 \end{bmatrix} + \sin(3t) \begin{bmatrix} 0 \\ 1 \end{bmatrix} \end{pmatrix}$

☐ $\mathbf{x}(t) = C_1 e^{3t} \begin{pmatrix} \cos(3t) \begin{bmatrix} 1 \\ 2 \end{bmatrix} + \sin(3t) \begin{bmatrix} 0 \\ -1 \end{bmatrix} \end{pmatrix} + C_2 e^{3t} \begin{pmatrix} \cos(3t) \begin{bmatrix} -1 \\ 0 \end{bmatrix} - \sin(3t) \begin{bmatrix} 1 \\ 2 \end{bmatrix} \end{pmatrix}$

☐ $\mathbf{x}(t) = C_1 e^{3t} \begin{pmatrix} \cos(3t) \begin{bmatrix} 0 \\ 1 \end{bmatrix} - \sin(3t) \begin{bmatrix} -1 \\ 0 \end{bmatrix} \end{pmatrix} + C_2 e^{3t} \begin{pmatrix} \cos(3t) \begin{bmatrix} -1 \\ 0 \end{bmatrix} + \sin(3t) \begin{bmatrix} 0 \\ 1 \end{bmatrix} \end{pmatrix}$

☐ $\mathbf{x}(t) = C_1 e^{3t} \begin{pmatrix} \cos(3t) \begin{bmatrix} 1 \\ 0 \end{bmatrix} - \sin(3t) \begin{bmatrix} -1 \\ 0 \end{bmatrix} \end{pmatrix} + C_2 e^{3t} \begin{pmatrix} \cos(3t) \begin{bmatrix} 0 \\ 1 \end{bmatrix} + \sin(3t) \begin{bmatrix} 0 \\ -1 \end{bmatrix} \end{pmatrix}$

☐ $\mathbf{x}(t) = C_1 e^{3t} \begin{pmatrix} \cos(3t) \begin{bmatrix} 0 \\ 1 \end{bmatrix} - \sin(3t) \begin{bmatrix} 1 \\ 2 \end{bmatrix} \end{pmatrix} + C_2 e^{3t} \begin{pmatrix} \cos(3t) \begin{bmatrix} 1 \\ 2 \end{bmatrix} + \sin(3t) \begin{bmatrix} 0 \\ 1 \end{bmatrix} \end{pmatrix}$

Find the general solution to the system $\mathbf{x}' = A \mathbf{x}$ where A is the given matrix.

$$A = \begin{bmatrix} 2 & 2 & 4 \\ 0 & 0 & -4 \\ 0 & 2 & 6 \end{bmatrix}$$

☐ $\mathbf{x}(t) = C_1 e^{2t} \begin{bmatrix} 1 \\ -1 \\ 1 \end{bmatrix} + C_2 e^{2t} \begin{bmatrix} 0 \\ 4 \\ -2 \end{bmatrix} + C_3 e^{-4t} \begin{bmatrix} 1 \\ 0 \\ 0 \end{bmatrix}$

☐ $\mathbf{x}(t) = C_1 e^{2t} \begin{bmatrix} 1 \\ -1 \\ 1 \end{bmatrix} + C_2 e^{2t} \begin{bmatrix} 0 \\ 4 \\ -2 \end{bmatrix} + C_3 e^{4t} \begin{bmatrix} 1 \\ 0 \\ 0 \end{bmatrix}$

☐ $\mathbf{x}(t) = C_1 e^{2t} \begin{bmatrix} 1 \\ 0 \\ 0 \end{bmatrix} + C_2 e^{2t} \begin{bmatrix} 0 \\ 4 \\ -2 \end{bmatrix} + C_3 e^{4t} \begin{bmatrix} 1 \\ -1 \\ 1 \end{bmatrix}$

☐ $\mathbf{x}(t) = C_1 e^{-2t} \begin{bmatrix} 1 \\ -1 \\ 1 \end{bmatrix} + C_2 e^{-2t} \begin{bmatrix} 1 \\ 0 \\ 0 \end{bmatrix} + C_3 e^{4t} \begin{bmatrix} 0 \\ 4 \\ -2 \end{bmatrix}$

☐ $\mathbf{x}(t) = C_1 e^{-2t} \begin{bmatrix} 1 \\ 0 \\ 0 \end{bmatrix} + C_2 e^{-2t} \begin{bmatrix} 1 \\ -1 \\ 1 \end{bmatrix} + C_3 e^{4t} \begin{bmatrix} 1 \\ -1 \\ 1 \end{bmatrix}$

Find the general solution to the system $\mathbf{x}' = A \mathbf{x}$ where A is the given matrix.

$$A = \begin{bmatrix} 0 & 1 & 0 \\ 0 & 0 & 1 \\ -12 & -16 & -7 \end{bmatrix}$$

☐ $\mathbf{x}(t) = C_1 e^{-2t} \begin{bmatrix} 1 \\ -2 \\ 4 \end{bmatrix} + C_2 \left(e^{-2t} \begin{bmatrix} 1 \\ -2 \\ 4 \end{bmatrix} + t e^{-2t} \begin{bmatrix} 0 \\ 1 \\ -4 \end{bmatrix} \right) + C_3 e^{-3t} \begin{bmatrix} 1 \\ -3 \\ 9 \end{bmatrix}$

☐ $\mathbf{x}(t) = C_1 e^{-2t} \begin{bmatrix} 1 \\ -2 \\ 4 \end{bmatrix} + C_2 \left(e^{-2t} \begin{bmatrix} 0 \\ 1 \\ -4 \end{bmatrix} + t e^{-2t} \begin{bmatrix} 1 \\ -2 \\ 4 \end{bmatrix} \right) + C_3 e^{-3t} \begin{bmatrix} 1 \\ -3 \\ 9 \end{bmatrix}$

☐ $\mathbf{x}(t) = C_1 e^{-2t} \begin{bmatrix} 1 \\ -2 \\ 4 \end{bmatrix} + C_2 e^{-2t} \begin{bmatrix} 0 \\ 1 \\ -4 \end{bmatrix} + C_3 e^{-3t} \begin{bmatrix} 1 \\ -3 \\ 9 \end{bmatrix}$

☐ $\mathbf{x}(t) = C_1 e^{2t} \begin{bmatrix} 1 \\ -2 \\ 4 \end{bmatrix} + C_2 \left(e^{2t} \begin{bmatrix} 0 \\ 1 \\ -4 \end{bmatrix} + t e^{2t} \begin{bmatrix} 1 \\ -2 \\ 4 \end{bmatrix} \right) + C_3 e^{3t} \begin{bmatrix} 1 \\ -3 \\ 9 \end{bmatrix}$

☐ $\mathbf{x}(t) = C_1 e^{-2t} \begin{bmatrix} 0 \\ 1 \\ -4 \end{bmatrix} + C_2 \left(e^{-2t} \begin{bmatrix} 0 \\ 1 \\ -4 \end{bmatrix} + t e^{-2t} \begin{bmatrix} 1 \\ -2 \\ 4 \end{bmatrix} \right) + C_3 e^{-3t} \begin{bmatrix} 1 \\ -3 \\ 9 \end{bmatrix}$

